Towards compositional models (#54)
* extract Signature from Builtin, rename Builtin to Model

* control

* int_model.v

* simple_int_model

* simple_list_functor

* model_of_relaxed

* bool_relaxed_model

* int_relaxed_model

* list_relaxed_functor

* example_list_int_model_1

* information_flow_functor

* information_flow_functor_trait

* WIP

* IFCRelaxedModelTrait1

* WIP

* eval_et_extensive_Some

* fix try_match_lhs_with_sc_complete

* WIP old stuff

* Expression2_countable

* eval_et_strip_helper

* thy_lhs_match_one_None

* fix naive_interpreter_sound

* WIP

* minor

* WIP

* minor, build coq-minuska

* run standalone tests

* remove `bench-coq` and `languages-in-coq`

* remove generated file

minuska/lib/micoqprint.ml
@@ -265,6 +265,8 @@ let print_definition
   def oux =
     let _ = def in
     fprintf oux "Require Import Minuska.pval_ocaml_binding %s %s Minuska.default_everything.\n"  (get_primitive_value_algebra name_of_builtins).pvae_coq_import (get_pi name_of_pi).pie_coq_import;
+    fprintf oux "Definition mysignature := (bi_signature MyUnit %s).\n" (get_primitive_value_algebra name_of_builtins).pvae_coq_entity_name;
+    fprintf oux "#[global] Existing Instance mysignature.\n";
     fprintf oux "Definition mybeta := (bi_beta MyUnit %s).\n" (get_primitive_value_algebra name_of_builtins).pvae_coq_entity_name;
     fprintf oux "#[global] Existing Instance mybeta.\n";
     fprintf oux "Definition my_program_info := %s.\n" (get_pi name_of_pi).pie_coq_entity_name;
