coq-minuska/theories/builtin/bool_model.v
@@ -1,0 +1,174 @@
+From Minuska Require Import
+    prelude
+    spec
+    bool_signature
+    model_traits
+    model_algebra
+    (* model_functor *)
+.
+
+Definition bool_carrier := bool.
+(* 
+#[export]
+Instance bool_carrier__with_bool_trait
+    :
+    WithBoolTrait bool_carrier
+:= {|
+    wbt_inject_bool := fun x => x ;
+|}. *)
+
+Definition bool_function_interp
+    {symbol : Type}
+    {symbols : Symbols symbol}
+    (NondetValue : Type)
+    (Carrier : Type)
+    {Cbool : Injection bool Carrier}
+    {Cerr : Injection ErrT Carrier}
+    (asb : Carrier -> option bool)
+:
+    BoolFunSymbol ->
+    NondetValue ->
+    list (@TermOver' symbol Carrier) ->
+    @TermOver' symbol Carrier
+:=
+    fun f nd args =>
+    match f with
+    | bool_fun_true => t_over (inject bool Carrier true)
+    | bool_fun_false => t_over (inject bool Carrier false)
+    | bool_fun_neg =>
+        match args with
+        | (t_over x1)::[] =>
+            match (asb x1) with
+            | Some true => t_over (inject bool Carrier false)
+            | Some false => t_over (inject bool Carrier true)
+            | None => t_over (inject ErrT Carrier et_error)
+            end
+        | _ => t_over (inject ErrT Carrier et_error)
+        end
+    | bool_fun_and =>
+        match args with
+        | (t_over (x1))::(t_over (x2))::[] =>
+            match (asb x1),(asb x2) with
+            | (Some b1), (Some b2) =>
+                t_over (inject bool Carrier (andb b1 b2))
+            | _,_ => t_over (inject ErrT Carrier et_error)
+            end
+        | _ => t_over (inject ErrT Carrier et_error)
+        end
+    | bool_fun_or =>
+        match args with
+        | (t_over (x1))::(t_over (x2))::[] =>
+            match (asb x1),(asb x2) with
+            | (Some b1), (Some b2) =>
+                t_over (inject bool Carrier (orb b1 b2))
+            | _,_ => t_over (inject ErrT Carrier et_error)
+            end
+        | _ => t_over (inject ErrT Carrier et_error)
+        end
+    | bool_fun_iff =>
+        match args with
+        | (t_over (x1))::(t_over (x2))::[] =>
+            match (asb x1),(asb x2) with
+            | (Some b1), (Some b2) =>
+                t_over (inject bool Carrier (eqb b1 b2))
+            | _, _ => t_over (inject ErrT Carrier et_error)
+            end
+        | _ => t_over (inject ErrT Carrier et_error)
+        end
+    | bool_fun_xor =>
+        match args with
+        | (t_over (x1))::(t_over (x2))::[] =>
+            match (asb x1),(asb x2) with
+            | (Some b1), (Some b2) =>
+                t_over (inject bool Carrier (negb (eqb b1 b2)))
+            | _, _ => t_over (inject ErrT Carrier et_error)
+            end
+        | _ => t_over (inject ErrT Carrier et_error)
+        end
+    end
+.
+
+Definition bool_predicate_interp
+    {symbol : Type}
+    {symbols : Symbols symbol}
+    (NondetValue : Type)
+    (Carrier : Type)
+    (asb : Carrier -> option bool)
+:
+    BoolPredSymbol ->
+    NondetValue ->
+    list (@TermOver' symbol Carrier) ->
+    bool
+:=
+    fun p nv args =>
+    match p with
+    | bool_pred_is => 
+        match args with
+        | (t_over x1)::[] =>
+            match (asb x1) with
+            | Some _ => true
+            | _ => false
+            end
+        | _ => false
+        end
+    | bool_pred_is_false =>
+        match args with
+        | (t_over x1)::[] =>
+            match (asb x1) with
+            | Some false => true
+            | _ => false
+            end
+        | _ => false
+        end
+    | bool_pred_is_true =>
+        match args with
+        | (t_over x1)::[] =>
+            match (asb x1) with
+            | Some true => true
+            | _ => false
+            end
+        | _ => false
+        end
+    end
+.
+
+Definition bool_model_over
+    (symbol : Type)
+    (symbols : Symbols symbol)
+    (NondetValue : Type)
+    (Carrier : Type)
+    (Cbool : Injection bool Carrier)
+    (Cerr : Injection ErrT Carrier)
+    (asb : Carrier -> option bool)
+    :
+    @ModelOver symbol symbols bool_signature NondetValue Carrier
+:= {|
+    builtin_function_interp := fun (f : @builtin_function_symbol bool_signature) => bool_function_interp NondetValue Carrier asb f;
+    builtin_predicate_interp := fun (p : @builtin_predicate_symbol bool_signature) => bool_predicate_interp NondetValue Carrier asb p;
+|}.
+
+Definition bool_relaxed_model
+    (symbol : Type)
+    (symbols : Symbols symbol)
+    (NondetValue : Type)
+    :
+    RelaxedModel bool_signature NondetValue ErrT
+:= {|
+    rm_carrier := bool_carrier ;
+    rm_model_over :=
+        fun (Carrier : Type)
+            (inja : Injection ErrT Carrier)
+            (injb : ReversibleInjection bool_carrier Carrier)
+            => bool_model_over symbol symbols NondetValue Carrier
+                (@ri_injection _ _ injb)
+                inja
+                (@ri_reverse _ _ injb)
+|}.
+
+(* Definition bool_model
+    (symbol : Type)
+    (symbols : Symbols symbol)
+    (NondetValue : Type)
+:=
+    model_of_relaxed (bool_relaxed_model symbol symbols NondetValue)
+. *)
