coq-minuska/theories/builtin/bool_signature.v
@@ -1,0 +1,74 @@
+From Minuska Require Import
+    prelude
+    spec
+.
+
+Variant BoolFunSymbol :=
+| bool_fun_true
+| bool_fun_false
+| bool_fun_neg
+| bool_fun_and
+| bool_fun_or
+| bool_fun_iff
+| bool_fun_xor
+.
+
+Variant BoolPredSymbol :=
+| bool_pred_is
+| bool_pred_is_false
+| bool_pred_is_true
+.
+
+#[local]
+Instance BoolFunSymbol_eqdec : EqDecision BoolFunSymbol.
+Proof.
+    ltac1:(solve_decision).
+Defined.
+
+#[local]
+Instance BoolPredSymbol_eqdec : EqDecision BoolPredSymbol.
+Proof.
+    ltac1:(solve_decision).
+Defined.
+
+#[local]
+Program Instance BoolFunSymbol_fin : Finite BoolFunSymbol := {|
+    enum := [
+        bool_fun_true;
+        bool_fun_false;
+        bool_fun_neg;
+        bool_fun_and;
+        bool_fun_or;
+        bool_fun_iff;
+        bool_fun_xor
+    ]
+|}.
+Next Obligation.
+    (repeat constructor); ltac1:(set_solver).
+Qed.
+Next Obligation.
+    destruct x; ltac1:(set_solver).
+Qed.
+Fail Next Obligation.
+
+
+#[local]
+Program Instance BoolPredSymbol_fin : Finite BoolPredSymbol := {|
+    enum := [
+        bool_pred_is;
+        bool_pred_is_false;
+        bool_pred_is_true
+    ]
+|}.
+Next Obligation.
+    (repeat constructor); ltac1:(set_solver).
+Qed.
+Next Obligation.
+    destruct x; ltac1:(set_solver).
+Qed.
+Fail Next Obligation.
+
+Definition bool_signature : Signature := {|
+    builtin_function_symbol := BoolFunSymbol ;
+    builtin_predicate_symbol := BoolPredSymbol ;
+|}.
