coq-minuska/theories/builtin/example_list_int_model.v
@@ -1,0 +1,25 @@
+From Minuska Require Import
+    prelude
+    spec
+    model_algebra
+    model_traits
+    builtin.list_signature
+    builtin.bool_model
+    builtin.int_model
+    builtin.list_model
+.
+
+
+Example example_list_int_model_1
+    {symbol : Type}
+    {symbols : Symbols symbol}
+    (NondetValue : Type)
+    :
+    Model list_signature NondetValue
+:=
+    model_of_relaxed (
+        rmf_apply list_relaxed_functor (
+            int_relaxed_model symbol symbols NondetValue
+        )
+    )
+.
