coq-minuska/theories/builtin/information_flow_functor.v
@@ -1,0 +1,492 @@
+From Minuska Require Import
+    prelude
+    spec
+    model_algebra
+    model_traits
+    properties
+.
+
+From stdpp Require Import decidable.
+
+Class IFLattice (TagType : Type) := {
+    ifl_meet :
+        TagType -> TagType -> TagType
+    ;
+    ifl_meet_assoc ::
+        Assoc (=) ifl_meet
+    ;
+    ifl_meet_comm ::
+        Comm (=) ifl_meet
+    ;
+
+    ifl_join :
+        TagType -> TagType -> TagType
+    ;
+    ifl_join_assoc ::
+        Assoc (=) ifl_join
+    ;
+    ifl_join_comm ::
+        Comm (=) ifl_join
+    ;
+
+    ifl_absorb_1 :
+        forall a b, ifl_join a (ifl_meet a b) = a
+    ;
+
+    ifl_absorb_2 :
+        forall a b, ifl_meet a (ifl_join a b) = a
+    ;
+
+    ifl_bot : TagType ;
+
+    ifl_join_bot :
+        forall a,
+        ifl_join ifl_bot a = a
+    ;
+
+    ifl_top : TagType ; 
+
+    ifl_meet_top :
+        forall a,
+        ifl_meet ifl_top a = a
+    ;
+}.
+
+
+Class IFCRelaxedModelTrait0
+    (TagType : Type)
+    {_E : EqDecision TagType}
+    {_C : Countable TagType}
+    {symbol : Type}
+    {symbols : Symbols symbol}
+    {signature : Signature}
+    {NondetValue : Type}
+    {FromT : Type}
+    {_EF : EqDecision FromT}
+    (Morig : RelaxedModel signature NondetValue FromT)
+    (Miflow : RelaxedModel signature NondetValue FromT)
+:= {
+    ifc_tagged :
+        @rm_carrier _ _ _ _ _ Morig ->
+        gset TagType ->
+        @rm_carrier _ _ _ _ _ Miflow
+    ;
+    ifc_get_tags :
+        @rm_carrier _ _ _ _ _ Miflow ->
+        gset TagType
+    ;
+    ifc_get_pure :
+        @rm_carrier _ _ _ _ _ Miflow ->
+        @rm_carrier _ _ _ _ _ Morig
+    ;
+
+    ifc_get_tags_of_tagged :
+        forall c tags,
+            ifc_get_tags (ifc_tagged c tags) = tags ;
+    
+    ifc_get_pure_of_tagged :
+        forall c tags,
+            ifc_get_pure (ifc_tagged c tags) = c ;
+}.
+
+Program Definition information_flow_functor
+    (TagType : Type)
+    {_E : EqDecision TagType}
+    {_C : Countable TagType}
+    :
+    RelaxedModelFunctorT void
+:= {|
+    rmf_signature := fun signature => signature ;
+    rmf_nondet := fun ND => ND ;
+
+    rmf_model :=
+        fun (signature : Signature)
+            (NondetValue : Type)
+            (symbol : Type)
+            (symbols : Symbols symbol)
+            M
+        => 
+        {|
+            rm_carrier := ((rm_carrier _ _ _ M)*(gset TagType)) ;
+            rm_model_over :=
+                fun
+                    (Carrier : Type)
+                    (inja : Injection void Carrier)
+                    (injb : ReversibleInjection _ Carrier)
+                =>
+                let myinj := (rinj_compose injb ({| 
+                    ri_injection := {| inject := fun a => (a,∅) |} ;
+                    ri_reverse := fun b => Some b.1
+                |})) in
+                {|
+                    builtin_function_interp :=
+                        fun
+                            (f : @builtin_function_symbol signature)
+                            (nv : NondetValue)
+                            l
+                        =>  @spec.builtin_function_interp _ _ _ _ _
+                            (@rm_model_over _ _ _ _ _ M Carrier inja 
+                                myinj
+                            )
+                            f
+                            nv
+                            l
+                    ;
+
+                    builtin_predicate_interp :=
+                        fun
+                            (p : @builtin_predicate_symbol signature)
+                            (nv : NondetValue)
+                            l
+                        =>  @spec.builtin_predicate_interp _ _ _ _ _
+                            (@rm_model_over _ _ _ _ _ M Carrier inja 
+                                myinj
+                            )
+                            p
+                            nv
+                            l
+                    ;
+                |}
+        |}  ;
+|}.
+Next Obligation.
+    intros.
+    ltac1:(unshelve(eapply prod_eq_dec)).
+    apply rm_carrier_eqdec.
+Defined.
+Next Obligation.
+    intros. simpl in *.
+    destruct M.
+    apply _.
+Defined.
+Next Obligation.
+    intros. simpl in *. ltac1:(simplify_eq/=). reflexivity.
+Qed.
+Fail Next Obligation.
+
+Definition information_flow_functor_tagged
+    (TagType : Type)
+    {_E : EqDecision TagType}
+    {_C : Countable TagType}
+    {symbol : Type}
+    {symbols : Symbols symbol}
+    {signature : Signature}
+    {NondetValue : Type}
+    (M : @RelaxedModel symbol symbols signature NondetValue void)
+    (c : @rm_carrier _ _ _ _ _ M)
+    (tags : gset TagType)
+    :
+    @rm_carrier _ _ _ _ _ (rmf_apply (information_flow_functor TagType) M)
+:=
+     (c,tags)
+.
+
+Definition information_flow_functor_get_tags
+    (TagType : Type)
+    {_E : EqDecision TagType}
+    {_C : Countable TagType}
+    {symbol : Type}
+    {symbols : Symbols symbol}
+    {signature : Signature}
+    {NondetValue : Type}
+    (M : @RelaxedModel symbol symbols signature NondetValue void)
+    (c' : @rm_carrier _ _ _ _ _ (rmf_apply (information_flow_functor TagType) M))
+    :
+    gset TagType
+:=
+    c'.2
+.
+
+Definition information_flow_functor_get_pure
+    (TagType : Type)
+    {_E : EqDecision TagType}
+    {_C : Countable TagType}
+    {symbol : Type}
+    {symbols : Symbols symbol}
+    {signature : Signature}
+    {NondetValue : Type}
+    (M : @RelaxedModel symbol symbols signature NondetValue void)
+    (c' : @rm_carrier _ _ _ _ _ (rmf_apply (information_flow_functor TagType) M))
+    :
+    @rm_carrier _ _ _ _ _ M
+:=
+    c'.1
+.
+
+#[export]
+Program Instance information_flow_functor_trait
+    (TagType : Type)
+    {_E : EqDecision TagType}
+    {_C : Countable TagType}
+    {symbol : Type}
+    {symbols : Symbols symbol}
+    {signature : Signature}
+    {NondetValue : Type}
+    (M : @RelaxedModel symbol symbols signature NondetValue void)
+    :
+    IFCRelaxedModelTrait0 TagType M (rmf_apply (information_flow_functor TagType) M)
+:= {|
+    ifc_tagged := information_flow_functor_tagged TagType M ;
+    ifc_get_tags := information_flow_functor_get_tags TagType M;
+    ifc_get_pure := information_flow_functor_get_pure TagType M;
+|}.
+Next Obligation.
+    intros.
+    simpl.
+    reflexivity.
+Qed.
+Next Obligation.
+    intros.
+    simpl.
+    reflexivity.
+Qed.
+Fail Next Obligation.
+
+Definition eval_predicate_in_orig
+    {TagType : Type}
+    {_E : EqDecision TagType}
+    {_C : Countable TagType}
+    {symbol : Type}
+    {symbols : Symbols symbol}
+    {signature : Signature}
+    {NondetValue : Type}
+    {FromT : Type}
+    {_EF : EqDecision FromT}
+    {Morig : RelaxedModel signature NondetValue FromT}
+    {Miflow : RelaxedModel signature NondetValue FromT}
+    (trait0 : IFCRelaxedModelTrait0 TagType Morig Miflow)
+    (Carrier : Type)
+    (inja : Injection FromT Carrier)
+    (injb : ReversibleInjection (@rm_carrier _ _ _ _ _ Morig) Carrier)
+    (p : builtin_predicate_symbol)
+    (nv : NondetValue)
+    (args : list (TermOver' (@rm_carrier _ _ _ _ _ Miflow)))
+:=
+    let args' : list (TermOver' (@rm_carrier _ _ _ _ _ Morig)) := (list_fmap _ _ (TermOver'_map ifc_get_pure) args) in
+    let args'' : list (TermOver' Carrier) := list_fmap _ _ (TermOver'_map (@inject _ _ (@ri_injection _ _ injb))) args' in
+    @builtin_predicate_interp _ _ _ _ _ (@rm_model_over _ _ signature _ _ Morig Carrier inja injb) p nv args''
+.
+
+Definition eval_predicate_in_iflow
+    {TagType : Type}
+    {_E : EqDecision TagType}
+    {_C : Countable TagType}
+    {symbol : Type}
+    {symbols : Symbols symbol}
+    {signature : Signature}
+    {NondetValue : Type}
+    {FromT : Type}
+    {_EF : EqDecision FromT}
+    {Morig : RelaxedModel signature NondetValue FromT}
+    {Miflow : RelaxedModel signature NondetValue FromT}
+    (trait0 : IFCRelaxedModelTrait0 TagType Morig Miflow)
+    (Carrier : Type)
+    (inja : Injection FromT Carrier)
+    (injb : ReversibleInjection (@rm_carrier _ _ _ _ _ Miflow) Carrier)
+    (p : builtin_predicate_symbol)
+    (nv : NondetValue)
+    (args : list (TermOver' (@rm_carrier _ _ _ _ _ Miflow)))
+:=
+    let args' := (TermOver'_map (@inject _ _ (@ri_injection _ _ injb))) <$> args in
+    @builtin_predicate_interp _ _ _ _ _ (@rm_model_over _ _ signature _ _ Miflow Carrier inja injb) p nv args'
+.
+
+
+Definition eval_function_in_orig
+    {TagType : Type}
+    {_E : EqDecision TagType}
+    {_C : Countable TagType}
+    {symbol : Type}
+    {symbols : Symbols symbol}
+    {signature : Signature}
+    {NondetValue : Type}
+    {FromT : Type}
+    {_EF : EqDecision FromT}
+    {Morig : RelaxedModel signature NondetValue FromT}
+    {Miflow : RelaxedModel signature NondetValue FromT}
+    (trait0 : IFCRelaxedModelTrait0 TagType Morig Miflow)
+    (Carrier : Type)
+    (inja : Injection FromT Carrier)
+    (injb : ReversibleInjection (@rm_carrier _ _ _ _ _ Morig) Carrier)
+    (f : builtin_function_symbol)
+    (nv : NondetValue)
+    (args : list (TermOver' (@rm_carrier _ _ _ _ _ Miflow)))
+    :
+    TermOver' Carrier
+:=
+    let args' : list (TermOver' (@rm_carrier _ _ _ _ _ Morig)) := (list_fmap _ _ (TermOver'_map ifc_get_pure) args) in
+    let args'' : list (TermOver' Carrier) := list_fmap _ _ (TermOver'_map (@inject _ _ (@ri_injection _ _ injb))) args' in
+    @builtin_function_interp _ _ _ _ _ (@rm_model_over _ _ signature _ _ Morig Carrier inja injb) f nv args''
+.
+
+Definition eval_function_in_iflow
+    {TagType : Type}
+    {_E : EqDecision TagType}
+    {_C : Countable TagType}
+    {symbol : Type}
+    {symbols : Symbols symbol}
+    {signature : Signature}
+    {NondetValue : Type}
+    {FromT : Type}
+    {_EF : EqDecision FromT}
+    {Morig : RelaxedModel signature NondetValue FromT}
+    {Miflow : RelaxedModel signature NondetValue FromT}
+    (trait0 : IFCRelaxedModelTrait0 TagType Morig Miflow)
+    (Carrier : Type)
+    (inja : Injection FromT Carrier)
+    (injb : ReversibleInjection (@rm_carrier _ _ _ _ _ Miflow) Carrier)
+    (f : builtin_function_symbol)
+    (nv : NondetValue)
+    (args : list (TermOver' (@rm_carrier _ _ _ _ _ Miflow)))
+    :
+    TermOver' Carrier
+:=
+    let args' := (TermOver'_map (@inject _ _ (@ri_injection _ _ injb))) <$> args in
+    @builtin_function_interp _ _ _ _ _ (@rm_model_over _ _ signature _ _ Miflow Carrier inja injb) f nv args'
+.
+
+Program Definition TermOver'_rinj
+    {T A B : Type}
+    (i : ReversibleInjection A B)
+    :
+    ReversibleInjection (@TermOver' T A) (@TermOver' T B)
+:= {|
+    ri_injection := {| 
+        inject := TermOver'_map (@inject _ _ (@ri_injection _ _ i))
+    |} ;
+    ri_reverse := TermOver'_option_map ((@ri_reverse _ _ i)) ;
+|}.
+Next Obligation.
+    intros.
+    unfold Inj.
+    intros x.
+    induction x; intros y; destruct y; intros HH; simpl in *.
+    {
+        ltac1:(injection HH as HH).
+        apply (inject_inj) in HH.
+        subst a0.
+        reflexivity.
+    }
+    {
+        inversion HH.
+    }
+    {
+        inversion HH.
+    }
+    {
+        ltac1:(injection HH as HH).
+        subst s0.
+        f_equal.
+        revert l0 H0 H.
+        induction l; intros l0 H0 H.
+        {
+            destruct l0; simpl in *.
+            { reflexivity. }
+            {
+                inversion H0.
+            }
+        }
+        {
+            destruct l0; simpl in *.
+            {
+                inversion H0.
+            }
+            {
+                inversion H0; subst; clear H0.
+                rewrite Forall_cons_iff in H.
+                destruct H as [H4 H5].
+                f_equal.
+                {
+                    apply H4.
+                    apply H2.
+                }
+                {
+                    apply IHl.
+                    apply H3.
+                    apply H5.
+                }
+            }
+        }
+    }
+Qed.
+Next Obligation.
+    intros.
+    destruct i as [i1 i2 i3]; simpl in *.
+    induction from; simpl in *.
+    {
+        rewrite i3.
+        reflexivity.
+    }
+    {
+        revert H.
+        induction l; intros H; simpl in *.
+        {
+            reflexivity.
+        }
+        {
+            rewrite Forall_cons_iff in H.
+            destruct H as [H1 H2].
+            specialize (IHl H2).
+            clear H2.
+            ltac1:(simplify_option_eq).
+            reflexivity.
+        }
+    }
+Qed.
+Fail Next Obligation.
+
+Class IFCRelaxedModelTrait1
+    (TagType : Type)
+    {_SL : IFLattice TagType}
+    {_E : EqDecision TagType}
+    {_C : Countable TagType}
+    {symbol : Type}
+    {symbols : Symbols symbol}
+    {signature : Signature}
+    {NondetValue : Type}
+    {FromT : Type}
+    {_EF : EqDecision FromT}
+    (Morig : RelaxedModel signature NondetValue FromT)
+    (Miflow : RelaxedModel signature NondetValue FromT)
+:= {
+
+    ifc_0 :: IFCRelaxedModelTrait0 TagType Morig Miflow ;
+
+    ifc_pure_predicate:
+        forall
+            (Carrier Carrier' : Type)
+            (inja : Injection FromT Carrier)
+            (inja' : Injection FromT Carrier')
+            (injb : ReversibleInjection (@rm_carrier _ _ _ _ _ Morig) Carrier)
+            (injb' : ReversibleInjection (@rm_carrier _ _ _ _ _ Miflow) Carrier'),
+        forall
+            (p : builtin_predicate_symbol)
+            (nv : NondetValue)
+            args,
+        eval_predicate_in_iflow ifc_0 Carrier' inja' injb' p nv args
+        =
+        eval_predicate_in_orig ifc_0 Carrier inja injb p nv args
+    ;
+
+    ifc_pure_function:
+        forall
+            (Carrier Carrier' : Type)
+            (inja : Injection FromT Carrier)
+            (inja' : Injection FromT Carrier')
+            (injb : ReversibleInjection (@rm_carrier _ _ _ _ _ Morig) Carrier)
+            (injb' : ReversibleInjection (@rm_carrier _ _ _ _ _ Miflow) Carrier'),
+        forall
+            (f : builtin_function_symbol)
+            (nv : NondetValue)
+            args,
+        let r1 : TermOver' Carrier' := eval_function_in_iflow ifc_0 Carrier' inja' injb' f nv args in
+        let r2 : TermOver' Carrier := eval_function_in_orig ifc_0 Carrier inja injb f nv args in
+        match @ri_reverse _ _ (TermOver'_rinj injb) r2, @ri_reverse _ _ (TermOver'_rinj injb') r1 with
+        | Some r'2, Some r'1 => (r'2) = (TermOver'_map ifc_get_pure r'1)
+        | _,_ => True
+        end
+    ;
+}.
+
+
+(* TODO need "the rest" of the natural transformation *)
