coq-minuska/theories/builtin/int_model.v
@@ -1,0 +1,167 @@
+From Minuska Require Import
+    prelude
+    spec
+    bool_model
+    int_signature
+    model_traits
+    model_algebra
+    (* model_functor *)
+.
+
+Definition int_carrier := Z.
+
+Definition int_function_interp
+    {symbol : Type}
+    {symbols : Symbols symbol}
+    (NondetValue : Type)
+    (Carrier : Type)
+    {_WE : Injection ErrT Carrier}
+    {_WB : Injection bool Carrier}
+    {_WI : Injection Z Carrier}
+    (asi : Carrier -> option int_carrier)
+:
+    IntFunSymbol ->
+    NondetValue ->
+    list (@TermOver' symbol Carrier) ->
+    @TermOver' symbol  Carrier
+:=
+    fun f nd args =>
+    match f with
+    | int_plus =>
+        match args with
+        | (t_over x1)::(t_over x2)::[] =>
+            match (asi x1), (asi x2) with
+            | Some z1, Some z2 => t_over (inject Z Carrier (z1 + z2)%Z)
+            | _, _ => t_over (inject ErrT Carrier et_error)
+            end
+        | _ => t_over (inject ErrT Carrier et_error)
+        end
+    | int_minus =>
+        match args with
+        | (t_over x1)::(t_over x2)::[] =>
+            match (asi x1), (asi x2) with
+            | Some z1, Some z2 => t_over (inject Z Carrier (z1 - z2)%Z)
+            | _, _ => t_over (inject ErrT Carrier et_error)
+            end
+        | _ => t_over (inject ErrT Carrier et_error)
+        end
+    | int_uminus =>
+        match args with
+        | (t_over x1)::[] =>
+            match (asi x1) with
+            | Some z1 => t_over (inject Z Carrier (-z1)%Z)
+            | _ => t_over (inject ErrT Carrier et_error)
+            end
+        | _ => t_over (inject ErrT Carrier et_error)
+        end
+    | int_zero =>
+        match args with
+        | [] => t_over (inject Z Carrier 0%Z)
+        | _ => t_over (inject ErrT Carrier et_error)
+        end
+    | int_one =>
+        match args with
+        | [] => t_over (inject Z Carrier 1%Z)
+        | _ => t_over (inject ErrT Carrier et_error)
+        end
+    | int_eq =>
+        match args with
+        | (t_over x1)::(t_over x2)::[] =>
+            match (asi x1),(asi x2) with
+            | Some z1, Some z2 => t_over (inject bool Carrier (bool_decide (z1 = z2)%Z))
+            | _, _ => t_over (inject ErrT Carrier et_error)
+            end
+        | _ => t_over (inject ErrT Carrier et_error)
+        end
+    | int_le =>
+        match args with
+        | (t_over x1)::(t_over x2)::[] =>
+            match (asi x1),(asi x2) with
+            | Some z1, Some z2 => t_over (inject bool Carrier (bool_decide (z1 <= z2)%Z))
+            | _, _ => t_over (inject ErrT Carrier et_error)
+            end
+        | _ => t_over (inject ErrT Carrier et_error)
+        end
+    | int_lt =>
+        match args with
+        | (t_over x1)::(t_over x2)::[] =>
+            match (asi x1),(asi x2) with
+            | Some z1, Some z2 => t_over (inject bool Carrier (bool_decide (z1 < z2)%Z))
+            | _, _ => t_over (inject ErrT Carrier et_error)
+            end
+        | _ => t_over (inject ErrT Carrier et_error)
+        end
+
+    end
+.
+
+Definition int_predicate_interp
+    {symbol : Type}
+    {symbols : Symbols symbol}
+    (NondetValue : Type)
+    (Carrier : Type)
+    (asi : Carrier -> option int_carrier)
+:
+    IntPredSymbol ->
+    NondetValue ->
+    list (@TermOver' symbol Carrier) ->
+    bool
+:=
+    fun p nv args =>
+    match p with
+    | bool_pred_is =>
+        match args with
+        | (t_over x1)::[] =>
+            match (asi x1) with
+            | Some _ => true
+            | _ => false
+            end
+        | _ => false
+        end
+    end
+.
+
+Definition int_model_over
+    (symbol : Type)
+    (symbols : Symbols symbol)
+    (NondetValue : Type)
+    (Carrier : Type)
+    (_WE : Injection ErrT Carrier)
+    (_WB : Injection bool Carrier)
+    (_WI : Injection Z Carrier)
+    (asi : Carrier -> option int_carrier)
+    :
+    @ModelOver symbol symbols int_signature NondetValue Carrier
+:= {|
+    builtin_function_interp := fun (f : @builtin_function_symbol int_signature) => int_function_interp NondetValue Carrier asi f;
+    builtin_predicate_interp := fun (p : @builtin_predicate_symbol int_signature) => int_predicate_interp NondetValue Carrier asi p;
+|}.
+
+Definition int_relaxed_model
+    (symbol : Type)
+    (symbols : Symbols symbol)
+    (NondetValue : Type)
+    :
+    RelaxedModel int_signature NondetValue (ErrT+bool)
+:= {|
+    rm_carrier := int_carrier ;
+    rm_model_over :=
+        fun (Carrier : Type)
+            (inja : Injection (ErrT+bool) Carrier)
+            (injb : ReversibleInjection int_carrier Carrier)
+            => int_model_over symbol symbols NondetValue Carrier
+                {| inject := fun (e:ErrT) => @inject _ _ inja (inl e) |}
+                {| inject := fun (b:bool) => @inject _ _ inja (inr b) |}
+                (@ri_injection _ _ injb)
+                (@ri_reverse _ _ injb)
+|}.
+
+(* Definition int_model
+    (symbol : Type)
+    (symbols : Symbols symbol)
+    (NondetValue : Type)
+    : Model int_signature NondetValue
+:=
+    model_of_relaxed (int_relaxed_model symbol symbols NondetValue)
+. *)
+
