coq-minuska/theories/builtin/int_signature.v
@@ -1,0 +1,72 @@
+From Minuska Require Import
+    prelude
+    spec
+.
+
+Variant IntFunSymbol :=
+| int_plus
+| int_minus
+| int_uminus
+| int_zero
+| int_one
+| int_eq
+| int_le
+| int_lt
+.
+
+Variant IntPredSymbol :=
+| int_is
+.
+
+#[local]
+Instance IntFunSymbol_eqdec : EqDecision IntFunSymbol.
+Proof.
+    ltac1:(solve_decision).
+Defined.
+
+#[local]
+Instance IntPredSymbol_eqdec : EqDecision IntPredSymbol.
+Proof.
+    ltac1:(solve_decision).
+Defined.
+
+#[local]
+Program Instance IntFunSymbol_fin : Finite IntFunSymbol := {|
+    enum := [
+        int_plus;
+        int_minus;
+        int_uminus;
+        int_zero;
+        int_one;
+        int_eq;
+        int_le;
+        int_lt
+    ]
+|}.
+Next Obligation.
+    (repeat constructor); ltac1:(set_solver).
+Qed.
+Next Obligation.
+    destruct x; ltac1:(set_solver).
+Qed.
+Fail Next Obligation.
+
+#[local]
+Program Instance IntPredSymbol_fin : Finite IntPredSymbol := {|
+    enum := [
+        int_is
+    ]
+|}.
+Next Obligation.
+    (repeat constructor); ltac1:(set_solver).
+Qed.
+Next Obligation.
+    destruct x; ltac1:(set_solver).
+Qed.
+Fail Next Obligation.
+
+Definition int_signature : Signature := {|
+    builtin_function_symbol := IntFunSymbol ;
+    builtin_predicate_symbol := IntPredSymbol ;
+|}.
+
