coq-minuska/theories/builtin/list_model.v
@@ -1,0 +1,236 @@
+From Minuska Require Import
+    prelude
+    spec
+    model_functor
+    model_traits
+    list_signature
+    model_algebra
+    (* model_functor *)
+.
+
+Definition list_function_interp
+    (InnerT : Type)
+    (symbol : Type)
+    (symbols : Symbols symbol)
+    (NondetValue : Type)
+    (Carrier : Type)
+    (_WE : Injection ErrT Carrier)
+    (_WB : Injection bool Carrier)
+    (_WI : Injection InnerT Carrier)
+    (_WL : Injection (list InnerT) Carrier)
+    (asi : Carrier -> option (InnerT))
+    (asl : Carrier -> option (list InnerT))
+:
+    ListFunSymbol ->
+    NondetValue ->
+    list (@TermOver' symbol Carrier) ->
+    @TermOver' symbol  Carrier
+:=
+    fun f nd args =>
+    match f with
+    | list_nil =>
+        match args with
+        | [] => t_over (inject (list InnerT) Carrier [])
+        | _ => t_over (inject ErrT Carrier et_error)
+        end
+    | list_cons =>
+        match args with
+        | (t_over x1)::(t_over x2)::[] =>
+            match (asi x1), (asl x2) with
+            | Some v, Some l => t_over (inject (list InnerT) Carrier (v::l))
+            | _, _ => t_over (inject ErrT Carrier et_error)
+            end
+        | _ => t_over (inject ErrT Carrier et_error)
+        end
+    | list_head =>
+        match args with
+        | (t_over x1)::[] =>
+            match asl x1 with
+            | Some [] => t_over (inject ErrT Carrier et_error)
+            | Some (h::_) => t_over (inject InnerT Carrier h)
+            | _ => t_over (inject ErrT Carrier et_error)
+            end
+        | _ => t_over (inject ErrT Carrier et_error)
+        end
+    | list_tail =>
+        match args with
+        | (t_over x1)::[] =>
+            match asl x1 with
+            | Some [] => t_over (inject ErrT Carrier et_error)
+            | Some (_::t) => t_over (inject (list InnerT) Carrier t)
+            | _ => t_over (inject ErrT Carrier et_error)
+            end
+        | _ => t_over (inject ErrT Carrier et_error)
+        end
+    | list_is_nil =>
+        match args with
+        | (t_over x1)::[] =>
+            match (asl x1) with
+            | Some l => t_over (inject bool Carrier (bool_decide (l = [])))
+            | _ => t_over (inject ErrT Carrier et_error)
+            end
+        | _ => t_over (inject ErrT Carrier et_error)
+        end
+    end
+.
+
+Definition list_predicate_interp
+    (InnerT : Type)
+    (symbol : Type)
+    (symbols : Symbols symbol)
+    (NondetValue : Type)
+    (Carrier : Type)
+    (_WE : Injection ErrT Carrier)
+    (_WB : Injection bool Carrier)
+    (_WI : Injection InnerT Carrier)
+    (_WL : Injection (list InnerT) Carrier)
+    (asi : Carrier -> option (InnerT))
+    (asl : Carrier -> option (list InnerT))
+:
+    ListPredSymbol ->
+    NondetValue ->
+    list (@TermOver' symbol Carrier) ->
+    bool
+:=
+    fun p nd args =>
+    match p with
+    | list_is =>
+        match args with
+        | (t_over x1)::[] =>
+            match (asl x1) with
+            | Some _ => true
+            | _ => false
+            end
+        | _ => false
+        end
+    end
+.
+
+Variant simple_list_carrier (Inner : Type) :=
+| slc_inner (x : Inner)
+| slc_list (l : list Inner)
+.
+
+#[local]
+Instance simple_list_carrier__eqdec
+    (Inner : Type)
+    {_ : EqDecision Inner}
+    : EqDecision (simple_list_carrier Inner)
+.
+Proof.
+    ltac1:(solve_decision).
+Defined.
+
+#[local]
+Program Instance simple_list_carrier__countable
+    (Inner : Type)
+    {_ : EqDecision Inner}
+    {_ : Countable Inner}
+    : Countable (simple_list_carrier Inner) := {|
+    encode := fun slc =>
+        stdpp.countable.encode (
+            match slc with
+            | slc_inner _ x => inl x
+            | slc_list _ l => inr l
+            end
+        )
+    ;
+    decode := fun (p : positive) =>
+        match (@stdpp.countable.decode (Inner+(list Inner)) _ _ p) with
+        | Some (inl x) => Some (slc_inner _ x)
+        | Some (inr l) => Some (slc_list _ l)
+        | None => None
+        end
+|}.
+Next Obligation.
+    rewrite decode_encode.
+        ltac1:(repeat case_match; simplify_eq/=);
+        reflexivity.
+Qed.
+Fail Next Obligation.
+
+Program Definition list_relaxed_functor :
+    RelaxedModelFunctorT (ErrT+bool)
+:= {|
+    rmf_signature := fun _ => list_signature ;
+    rmf_nondet := fun ND => ND ;
+
+    rmf_model :=
+        fun (signature : Signature)
+            (NondetValue : Type)
+            (symbol : Type)
+            (symbols : Symbols symbol)
+            M
+        => 
+        {|
+            rm_carrier := (simple_list_carrier (rm_carrier _ _ _ M)) ;
+            rm_model_over :=
+                fun
+                    (Carrier : Type)
+                    (inja : Injection (ErrT+bool) Carrier)
+                    (injb : ReversibleInjection (simple_list_carrier (rm_carrier _ _ _ M)) Carrier)
+                => 
+                    let asi := (fun c =>
+                        match (@ri_reverse _ _ injb) c with Some d => (
+                            match d with
+                            | slc_inner _ d' => Some d'
+                            | _ => None
+                            end
+                        )
+                        | None => None end) in
+                    let asl := (fun c =>
+                        match (@ri_reverse _ _ injb) c with Some d => (
+                            match d with
+                            | slc_list _ d' => Some d'
+                            | _ => None
+                            end
+                        )
+                        | None => None end) in
+                let WL : Injection (list (rm_carrier signature NondetValue (ErrT + bool) M)) Carrier := {|
+                    inject := fun l => @inject _ _ (@ri_injection _ _ injb) (slc_list _ l)
+                |} in
+                let WI := {|
+                    inject := fun i => @inject _ _ (@ri_injection _ _ injb) (slc_inner _ i)
+                |} in
+                let WB := {|
+                    inject := fun b => @inject _ _ inja (inr b)                
+                |} in
+                let WE := {|
+                    inject := fun e => @inject _ _ inja (inl e)                
+                |} in
+                {|
+                    builtin_function_interp := fun (f : @builtin_function_symbol list_signature) => list_function_interp (rm_carrier _ _ _ M) symbol symbols NondetValue Carrier WE WB WI WL asi asl f;
+                    builtin_predicate_interp := fun (p : @builtin_predicate_symbol list_signature) => list_predicate_interp (rm_carrier _ _ _ M) symbol symbols NondetValue Carrier WE WB WI WL asi asl p;
+                |}
+        |}  ;
+|}.
+Next Obligation.
+    apply simple_list_carrier__eqdec.
+    apply rm_carrier_eqdec.
+Defined.
+Next Obligation.
+    (* Countable *)
+    destruct M.
+    apply _.
+Defined.
+Next Obligation.
+    apply inject_inj in H.
+    ltac1:(injection H as H).
+    exact H.
+Qed.
+Next Obligation.
+    apply inject_inj in H.
+    ltac1:(injection H as H).
+    exact H.
+Qed.
+Next Obligation.
+    apply inject_inj in H.
+    ltac1:(injection H as H).
+    exact H.
+Qed.
+Next Obligation.
+    destruct x,y; reflexivity.
+Qed.
+Fail Next Obligation.
+
+
