coq-minuska/theories/builtin/list_signature.v
@@ -1,0 +1,66 @@
+From Minuska Require Import
+    prelude
+    spec
+.
+
+Variant ListFunSymbol :=
+| list_nil
+| list_cons
+| list_head
+| list_tail
+| list_is_nil
+.
+
+Variant ListPredSymbol :=
+| list_is
+.
+
+#[local]
+Instance ListFunSymbol_eqdec : EqDecision ListFunSymbol.
+Proof.
+    ltac1:(solve_decision).
+Defined.
+
+#[local]
+Instance ListPredSymbol_eqdec : EqDecision ListPredSymbol.
+Proof.
+    ltac1:(solve_decision).
+Defined.
+
+#[local]
+Program Instance ListFunSymbol_fin : Finite ListFunSymbol := {|
+    enum := [
+        list_nil;
+        list_cons;
+        list_head;
+        list_tail;
+        list_is_nil
+    ]
+|}.
+Next Obligation.
+    (repeat constructor); ltac1:(set_solver).
+Qed.
+Next Obligation.
+    destruct x; ltac1:(set_solver).
+Qed.
+Fail Next Obligation.
+
+#[local]
+Program Instance ListPredSymbol_fin : Finite ListPredSymbol := {|
+    enum := [
+        list_is
+    ]
+|}.
+Next Obligation.
+    (repeat constructor); ltac1:(set_solver).
+Qed.
+Next Obligation.
+    destruct x; ltac1:(set_solver).
+Qed.
+Fail Next Obligation.
+
+Definition list_signature : Signature := {|
+    builtin_function_symbol := ListFunSymbol ;
+    builtin_predicate_symbol := ListPredSymbol ;
+|}.
+
