coq-minuska/theories/interpreter_results.v
@@ -77,122 +77,14 @@ Proof.
     }
 Qed.    
 
-Lemma wf2'_impl_wf2
+#[export]
+Instance RewritingTheory2_wf_dec
     {Σ : StaticModel}
-    {Act : Set}
-    (r : RewritingRule2 Act)
+    (Act : Set)
+    (Γ : list (RewritingRule2 Act))
     :
-    RewritingRule2_wf2' r -> 
-    RewritingRule2_wf2 r
+    Decision (RewritingTheory2_wf Γ)
 .
 Proof.
-    intros H.
-    unfold RewritingRule2_wf2' in H.
-    unfold RewritingRule2_wf2.
-    intros g ρ program nv Hfrom Hscs.
-    clear Hscs.
-    
-    unfold satisfies in Hfrom; simpl in Hfrom.
-    apply vars_of_sat_tobov in Hfrom.
-    assert (Hvtρ : vars_of (r_to r) ⊆ vars_of ρ).
-    {
-        eapply transitivity>[apply H|]. apply Hfrom.
-    }
-    clear H Hfrom.
-    apply TermOverExpression2_evalute_total_2 with (program := program) (nv := nv) in Hvtρ.
-    exact Hvtρ.
-Qed.
-
-Definition RewritingRule2_wf2_heuristics
-    {Σ : StaticModel}
-    {Act : Set}
-    (r : RewritingRule2 Act)
-    :
-    option (RewritingRule2_wf2 r)
-.
-Proof.
-    eapply option_map.
-    { apply wf2'_impl_wf2. }
-    unfold RewritingRule2_wf2'.
-    destruct (decide (vars_of (r_to r) ⊆ (vars_of (r_from r)))) as [H|H].
-    {
-        exact (Some H).
-    }
-    exact None.
-Defined.
-
-Definition RewritingRule2_wf_heuristics
-    {Σ : StaticModel}
-    {Act : Set}
-    (r : RewritingRule2 Act)
-    : option (RewritingRule2_wf r)
-.
-Proof.
-    unfold RewritingRule2_wf.
-    destruct (decide (vars_of (r_scs r) ⊆ (vars_of (r_from r)))) as [H|H].
-    {
-
-        assert (H2 := RewritingRule2_wf2_heuristics r).
-        unfold RewritingRule2_wf1.
-        destruct H2 as [H2|].
-        {
-            exact (Some (H, H2)).
-        }
-        exact None.
-    }
-    exact None.
-Defined.
-
-Definition RewritingTheory2_wf_heuristics
-    {Σ : StaticModel}
-    {Act : Set}
-    {_dAct : EqDecision Act}
-    (Γ : RewritingTheory2 Act)
-    : option (RewritingTheory2_wf Γ)
-.
-Proof.
-    unfold RewritingTheory2_wf.
-    induction Γ.
-    {
-        apply Some.
-        intros r Hr.
-        rewrite elem_of_nil in Hr.
-        inversion Hr.
-    }
-    {
-        destruct IHΓ as [IHΓ|].
-        {
-            assert (H := RewritingRule2_wf_heuristics a).
-            destruct H as [H|].
-            {
-                apply Some.
-                intros r Hr.
-                split.
-                {
-                    destruct (decide (r = a)).
-                    {
-                        subst. apply H.
-
-                    }
-                    {
-                        assert (r ∈ Γ) by (ltac1:(set_solver)).
-                        apply IHΓ; assumption.
-                    }
-                }
-                {
-                    destruct (decide (r = a)).
-                    {
-                        subst. apply H.
-
-                    }
-                    {
-                        assert (r ∈ Γ) by (ltac1:(set_solver)).
-                        apply IHΓ; assumption.
-                    }
-                }
-            }
-            exact None.
-        }
-        exact None.
-    }
+    apply _.
 Defined.
