coq-minuska/theories/model_algebra.v
@@ -1,0 +1,449 @@
+From Minuska Require Import
+    prelude
+    spec
+    signature_morphism
+.
+
+From Coq Require Import Logic.Eqdep_dec.
+
+#[local]
+Arguments builtin_function_symbol (Signature) : clear implicits.
+#[local]
+Arguments builtin_predicate_symbol (Signature) : clear implicits.
+#[local]
+Arguments builtin_function_interp {symbol} {symbols signature}
+  {NondetValue Carrier} (ModelOver) _ _ _
+.
+#[local]
+Arguments builtin_predicate_interp {symbol} {symbols signature}
+  {NondetValue Carrier} (ModelOver) _ _ _
+.
+
+Class Injection (FromT ToT : Type) := {
+    inject : FromT -> ToT ;
+    inject_inj :: Inj (=) (=) inject ;
+}.
+
+Arguments inject (FromT ToT) {Injection} _.
+
+Definition inj_compose {A B C : Type} (g : Injection B C) (f : Injection A B) := {|
+    inject := compose (@inject _ _ g) (@inject _ _ f) ;
+|}. 
+
+Program Definition inj_id (A : Type) : Injection A A :=
+{| inject := fun x => x; |}
+.
+Fail Next Obligation.
+
+(* Of course not.
+Program Definition inj_fst (A B : Type) : Injection (prod A B) A :=
+{|
+    inject := fst ;
+|}.
+Next Obligation.
+Fail Next Obligation. *)
+
+Class ReversibleInjection (FromT ToT : Type) := {
+    ri_injection :: Injection FromT ToT ;
+    ri_reverse : ToT -> option FromT ;
+    ri_reverse_pf : forall from,
+        ri_reverse (@inject FromT ToT ri_injection from) = Some from ;
+}.
+
+Program Definition rinj_compose
+    {A B C : Type}
+    (g : ReversibleInjection B C)
+    (f : ReversibleInjection A B)
+:= {|
+    ri_injection := inj_compose (@ri_injection _ _ g) (@ri_injection _ _ f) ;
+    ri_reverse := fun c =>
+        b ← (@ri_reverse _ _ g c);
+        (@ri_reverse _ _ f b)
+|}.
+Next Obligation.
+    rewrite ri_reverse_pf.
+    simpl.
+    rewrite ri_reverse_pf.
+    reflexivity.
+Qed.
+Fail Next Obligation.
+
+Program Definition rinj_id (A : Type) : ReversibleInjection A A := {|
+    ri_injection := {| inject := fun x => x; |};
+    ri_reverse := fun x => Some x;
+|}.
+Fail Next Obligation.
+
+Program Definition rinj_inl (A B : Type) : ReversibleInjection A (A+B) := {|
+    ri_injection := {| inject := inl; |} ;
+    ri_reverse := fun x => match x with inl x' => Some x' | _ => None end ;
+|}.
+Fail Next Obligation.
+
+Program Definition rinj_inr (A B : Type) : ReversibleInjection B (A+B) := {|
+    ri_injection := {| inject := inr; |} ;
+    ri_reverse := fun x => match x with inr x' => Some x' | _ => None end ;
+|}.
+Fail Next Obligation.
+
+Record RelaxedModel
+    {symbol : Type}
+    {symbols : Symbols symbol}
+    (signature : Signature)
+    (NondetValue : Type)
+    (FromT : Type)
+:= {
+    rm_carrier :
+        Type
+    ;
+    rm_carrier_eqdec :
+        EqDecision rm_carrier
+    ;
+    rm_carrier_countable :
+        Countable rm_carrier
+    ;
+    rm_model_over :
+        forall (Carrier : Type),
+        Injection FromT Carrier ->
+        ReversibleInjection rm_carrier Carrier ->
+        ModelOver signature NondetValue Carrier
+    ;
+}.
+
+Program Definition model_of_relaxed
+    {symbol : Type}
+    {symbols : Symbols symbol}
+    {signature : Signature}
+    {NondetValue : Type}
+    {FromT : Type}
+    {_EFT : EqDecision FromT}
+    {_CT : Countable FromT}
+    (RM : RelaxedModel signature NondetValue FromT)
+    :
+    Model signature NondetValue
+:= {|
+    builtin_value := sum FromT (rm_carrier _ _ _ RM) ;
+    builtin_model_over :=
+        rm_model_over signature NondetValue FromT RM
+        (sum FromT (rm_carrier _ _ _ RM))
+        {| inject := inl |}
+        {|
+            ri_injection := {| inject := inr |} ;
+            ri_reverse := fun x => match x with inr x' => Some x' | _ => None end ;
+        |}
+        
+|}.
+Next Obligation.
+    destruct RM as [c ed ov].
+    apply _.
+Defined.
+Next Obligation.
+    destruct RM.
+    apply _.
+Defined.
+Fail Next Obligation.
+
+Record RelaxedModelFunctorT (FromT : Type) := {
+    rmf_signature : Signature -> Signature ;
+    rmf_nondet : Type -> Type ;
+
+    rmf_model :
+        forall
+            (signature : Signature)
+            (NondetValue : Type)
+            {symbol : Type}
+            {symbols : Symbols symbol},
+            @RelaxedModel symbol symbols signature NondetValue FromT ->
+            (* (inja : Injection FromT Carrier) *)
+            (* (injb : ReversibleInjection (rmf_carrier Carrier) Carrier), *)
+            @RelaxedModel
+                symbol
+                symbols
+                (rmf_signature signature)
+                (rmf_nondet NondetValue)
+                FromT
+}.
+
+Definition rmf_apply
+    {FromT : Type}
+    (f : RelaxedModelFunctorT FromT)
+    {signature : Signature}
+    {NondetValue : Type}
+    {symbol : Type}
+    {symbols : Symbols symbol}
+    (M : @RelaxedModel symbol symbols signature NondetValue FromT)
+    :
+    @RelaxedModel
+        symbol
+        symbols
+        (rmf_signature _ f signature)
+        (rmf_nondet _ f NondetValue)
+        FromT
+:= 
+    rmf_model _ f _ _ M
+.
+
+(* 
+Definition rmf_apply
+    {symbol : Type}
+    {symbols : Symbols symbol}
+    (FromT : Type)
+    (f : RelaxedModelFunctorT FromT)
+    {signature : Signature}
+    {NondetValue : Type}
+    (x : RelaxedModel signature NondetValue FromT)
+    :
+    RelaxedModel (@rmf_signature _ f signature) (@rmf_nondet _ f NondetValue) FromT
+:= {|
+    rm_carrier := rmf_carrier _ f (@rm_carrier _ _ _ _ _ x) ;
+    rm_carrier_eqdec := rmf_carrier_eqdec _ f _ ((@rm_carrier_eqdec _ _ _ _ _ x)) ;
+    rm_model_over :=
+        fun (Carrier : Type)
+            (inja : Injection FromT Carrier)
+            (injb : ReversibleInjection _ Carrier)
+        => @rmf_model_over _ f signature NondetValue symbol symbols Carrier
+            (* inja *)
+            (* _ *)
+(*             
+            {|
+                ri_injection := {|
+                    inject := 0
+                    (* fun (a : (rmf_carrier FromT f (rm_carrier signature NondetValue FromT x))) => (@inject _ _ (@ri_injection _ _ injb) a) *)
+                    (* inject := @rmf_from _ f _ _ (@inject _ _ (@ri_injection _ _ injb)) *)
+                |}
+            |} *)
+            (* injb *)
+         ;
+
+|}. *)
+
+
+
+Definition model_reduction
+    (s1 s2 : Signature)
+    (μ : SignatureMorphism s1 s2)
+    (NV Carrier : Type)
+    {symbol : Type}
+    {symbols : Symbols symbol}
+    :
+    ModelOver s2 NV Carrier ->
+    ModelOver s1 NV Carrier
+:= fun m2 =>
+{|
+    builtin_function_interp :=
+        fun (f : builtin_function_symbol s1)
+            (nv : NV)
+            (args : list (@TermOver' symbol Carrier))
+        => spec.builtin_function_interp m2 (function_symbol_morphism μ f) nv args;
+
+    builtin_predicate_interp :=
+        fun (p : builtin_predicate_symbol s1)
+            (nv : NV)
+            (args : list (@TermOver' symbol Carrier))
+        => spec.builtin_predicate_interp m2 (predicate_symbol_morphism μ p) nv args;
+|}
+.
+
+Section sum.
+
+    Definition signature_sum (s1 s2 : Signature) : Signature := {|
+        builtin_function_symbol := sum (builtin_function_symbol s1) (builtin_function_symbol s2) ;
+        builtin_predicate_symbol := sum (builtin_predicate_symbol s1) (builtin_predicate_symbol s2) ;
+    |}.
+
+    Definition signature_sum_morphism_1_function
+        (s1 s2 : Signature)
+        : (builtin_function_symbol s1) -> (builtin_function_symbol (signature_sum s1 s2))
+    :=
+        fun f => inl f
+    .
+
+    Definition signature_sum_morphism_1_predicate
+        (s1 s2 : Signature)
+        : (builtin_predicate_symbol s1) -> (builtin_predicate_symbol (signature_sum s1 s2))
+    :=
+        fun f => inl f
+    .
+
+    Definition signature_sum_morphism_1 (s1 s2 : Signature)
+        : SignatureMorphism s1 (signature_sum s1 s2)
+    := {|
+        function_symbol_morphism := signature_sum_morphism_1_function s1 s2 ;
+        predicate_symbol_morphism := signature_sum_morphism_1_predicate s1 s2 ;
+    |}.
+
+
+    Definition signature_sum_morphism_2_function
+        (s1 s2 : Signature)
+        : (builtin_function_symbol s2) -> (builtin_function_symbol (signature_sum s1 s2))
+    :=
+        fun f => inr f
+    .
+
+    Definition signature_sum_morphism_2_predicate
+        (s1 s2 : Signature)
+        : (builtin_predicate_symbol s2) -> (builtin_predicate_symbol (signature_sum s1 s2))
+    :=
+        fun f => inr f
+    .
+
+    Definition signature_sum_morphism_2 (s1 s2 : Signature)
+        : SignatureMorphism s2 (signature_sum s1 s2)
+    := {|
+        function_symbol_morphism := signature_sum_morphism_2_function s1 s2 ;
+        predicate_symbol_morphism := signature_sum_morphism_2_predicate s1 s2 ;
+    |}.
+
+    #[export]
+    Program Instance signature_sum_morph_1_inj
+        (s1 s2 : Signature)
+        :
+        SMInj (signature_sum_morphism_1 s1 s2)
+    .
+    Fail Next Obligation.
+
+    #[export]
+    Program Instance signature_sum_morph_2_inj
+        (s1 s2 : Signature)
+        :
+        SMInj (signature_sum_morphism_2 s1 s2)
+    .
+    Fail Next Obligation.
+
+
+    Definition function_interp_sum
+        {symbol : Type}
+        {symbols : Symbols symbol}
+        (s1 s2 : Signature)
+        (NV Carrier : Type)
+        (m1 : ModelOver s1 NV Carrier)
+        (m2 : ModelOver s2 NV Carrier)
+        (f : @builtin_function_symbol (signature_sum s1 s2))
+        (nv : NV)
+        (args : list (@TermOver' symbol Carrier))
+        :
+        (@TermOver' symbol Carrier)
+    :=
+        match f with
+        | inl f' => @builtin_function_interp symbol symbols s1 NV Carrier m1 f' nv args
+        | inr f' => @builtin_function_interp symbol symbols s2 NV Carrier m2 f' nv args
+        end
+    .
+
+    Definition predicate_interp_sum
+        {symbol : Type}
+        {symbols : Symbols symbol}
+        (s1 s2 : Signature)
+        (NV Carrier : Type)
+        (m1 : ModelOver s1 NV Carrier)
+        (m2 : ModelOver s2 NV Carrier)
+        (p : @builtin_predicate_symbol (signature_sum s1 s2))
+        (nv : NV)
+        (args : list (@TermOver' symbol Carrier))
+        :
+        bool
+    :=
+        match p with
+        | inl p' => @builtin_predicate_interp symbol symbols s1 NV Carrier m1 p' nv args
+        | inr p' => @builtin_predicate_interp symbol symbols s2 NV Carrier m2 p' nv args
+        end
+    .
+
+    Definition modelover_sum
+        {symbol : Type}
+        {symbols : Symbols symbol}
+        (s1 s2 : Signature)
+        (NV : Type)
+        (Carrier : Type)
+        (m1 : ModelOver s1 NV Carrier)
+        (m2 : ModelOver s2 NV Carrier)
+    :
+        ModelOver (signature_sum s1 s2) NV Carrier
+    := {|
+        builtin_function_interp :=  function_interp_sum s1 s2 NV Carrier m1 m2;
+        builtin_predicate_interp :=  predicate_interp_sum s1 s2 NV Carrier m1 m2;
+    |}
+    .
+
+    Lemma modelover_sum_reduce_1
+        {symbol : Type}
+        {symbols : Symbols symbol}
+        (s1 s2 : Signature)
+        (NV : Type)
+        (Carrier : Type)
+        (m1 : ModelOver s1 NV Carrier)
+        (m2 : ModelOver s2 NV Carrier)
+    :
+        model_reduction
+            s1 (signature_sum s1 s2)
+            (signature_sum_morphism_1 s1 s2)
+            NV Carrier
+            (modelover_sum s1 s2 NV Carrier m1 m2)
+        = m1.
+    Proof.
+        unfold model_reduction.
+        destruct m1 as [f1 p1]; simpl in *.
+        destruct m2 as [f2 p2]; simpl in *.
+        f_equal.
+    Qed.
+
+    Lemma modelover_sum_reduce_2
+        {symbol : Type}
+        {symbols : Symbols symbol}
+        (s1 s2 : Signature)
+        (NV : Type)
+        (Carrier : Type)
+        (m1 : ModelOver s1 NV Carrier)
+        (m2 : ModelOver s2 NV Carrier)
+    :
+        model_reduction
+            s2 (signature_sum s1 s2)
+            (signature_sum_morphism_2 s1 s2)
+            NV Carrier
+            (modelover_sum s1 s2 NV Carrier m1 m2)
+        = m2.
+    Proof.
+        unfold model_reduction.
+        destruct m2; simpl in *.
+        f_equal.
+    Qed.
+
+
+End sum.
+
+Definition modelover_nv_lift 
+    {symbol : Type}
+    {symbols : Symbols symbol}
+    {signature: Signature}
+    {NV1 NV2 : Type}
+    {Carrier : Type}
+    (nvf : NV2 -> NV1)
+    (m : ModelOver signature NV1 Carrier)
+    :
+    ModelOver signature NV2 Carrier
+:= {|
+    builtin_function_interp :=
+        fun f nv args => @builtin_function_interp _ _ _ _ _ m f (nvf nv) args
+    ;
+    builtin_predicate_interp :=
+        fun p nv args => @builtin_predicate_interp _ _ _ _ _ m p (nvf nv) args
+    ;
+|}.
+
+(* 
+Definition modelover_carrier_lift 
+    {symbol : Type}
+    {symbols : Symbols symbol}
+    {signature: Signature}
+    {NV : Type}
+    {Carrier1 Carrier2 : Type}
+    (cf : ReversibleInjection Carrier1 Carrier2)
+    (m : ModelOver signature NV Carrier1)
+    :
+    ModelOver signature NV Carrier2
+:= {|
+    builtin_function_interp :=
+        fun f nv args => @builtin_function_interp _ _ _ _ _ m f nv ((TermOver'_map (@ri_reverse Carrier1 Carrier2 cf)) <$> args)
+|}.
+ *)
+
