coq-minuska/theories/model_traits.v
@@ -1,0 +1,71 @@
+From Minuska Require Import
+    prelude
+    spec
+    model_functor
+.
+
+Inductive ErrT :=
+| et_error
+.
+
+#[export]
+Instance ErrT_eqdec : EqDecision ErrT.
+Proof.
+    unfold RelDecision.
+    intros [] []. left. reflexivity.
+Defined.
+
+#[export]
+Program Instance ErrT_fin : Finite ErrT := {|
+    enum := [et_error] ;
+|}.
+Next Obligation.
+    (repeat constructor); ltac1:(set_solver).
+Qed.
+Next Obligation.
+    destruct x; ltac1:(set_solver).
+Qed.
+Fail Next Obligation.
+
+(* 
+Class WithErrTrait
+    {symbol : Type}
+    {symbols : Symbols symbol}
+    {my_signature : Signature}
+    {NondetValue : Type}
+    (M : Model my_signature NondetValue)
+:= {
+    inject_error :: CarrierInjection ErrT M ;
+}.
+
+Class WithBoolTrait
+    {symbol : Type}
+    {symbols : Symbols symbol}
+    {my_signature : Signature}
+    {NondetValue : Type}
+    (M : Model my_signature NondetValue)
+:= {
+    inject_bool :: CarrierInjection bool M ;
+}.
+
+Class WithIntTrait
+    {symbol : Type}
+    {symbols : Symbols symbol}
+    {my_signature : Signature}
+    {NondetValue : Type}
+    (M : Model my_signature NondetValue)
+:= {
+    inject_int :: CarrierInjection Z M ;
+}.
+
+Class WithListTrait (Inner : Type)
+    {symbol : Type}
+    {symbols : Symbols symbol}
+    {my_signature : Signature}
+    {NondetValue : Type}
+    (M : Model my_signature NondetValue)
+:= {
+    inject_list_inner :: CarrierInjection Inner M ;
+    inject_list :: CarrierInjection (list Inner) M ;
+}.
+ *)
