coq-minuska/theories/pval_ocaml_binding.v
@@ -8,14 +8,15 @@ From Minuska Require Import
 
 From Coq Require Import String ZArith.
 
-Record BuiltinInterface (NondetValue : Type) := {
-    bi_beta : Builtin (NondetValue : Type) ;
+Record BuiltinInterface (NondetValue : Type) := mkBuiltinInterface {
+    bi_signature : Signature ;
+    bi_beta : Model bi_signature (NondetValue : Type) ;
     bi_bindings : BuiltinsBinding ;
-    bi_inject_err : (@builtin_value _ _ NondetValue bi_beta) ;
-    bi_inject_bool : forall (Fret : option (@builtin_value _ _ NondetValue bi_beta) -> (@builtin_value _ _ NondetValue bi_beta)), bool -> (@builtin_value _ _ NondetValue bi_beta) ;
-    bi_inject_Z : forall (Fret : option (@builtin_value _ _ NondetValue bi_beta) -> (@builtin_value _ _ NondetValue bi_beta)), Z -> (@builtin_value _ _ NondetValue bi_beta) ;
-    bi_inject_string : forall (Fret : option (@builtin_value _ _ NondetValue bi_beta) -> (@builtin_value _ _ NondetValue bi_beta)), string -> (@builtin_value _ _ NondetValue bi_beta) ;
-    bi_eject : (@builtin_value _ _ NondetValue bi_beta) -> option (bool+(Z+(string+unit)))%type ;
+    bi_inject_err : (@builtin_value _ _ _ NondetValue bi_beta) ;
+    bi_inject_bool : forall (Fret : option (@builtin_value _ _ _ NondetValue bi_beta) -> (@builtin_value _ _ _ NondetValue bi_beta)), bool -> (@builtin_value _ _ _ NondetValue bi_beta) ;
+    bi_inject_Z : forall (Fret : option (@builtin_value _ _ _ NondetValue bi_beta) -> (@builtin_value _ _ _ NondetValue bi_beta)), Z -> (@builtin_value _ _ _ NondetValue bi_beta) ;
+    bi_inject_string : forall (Fret : option (@builtin_value _ _ _ NondetValue bi_beta) -> (@builtin_value _ _ _ NondetValue bi_beta)), string -> (@builtin_value _ _ _ NondetValue bi_beta) ;
+    bi_eject : (@builtin_value _ _ _ NondetValue bi_beta) -> option (bool+(Z+(string+unit)))%type ;
 }.
 
 Definition builtins_empty : BuiltinInterface MyUnit := {|
