coq-minuska/theories/signature_morphism.v
@@ -1,0 +1,30 @@
+From Minuska Require Import
+    prelude
+    spec
+.
+
+#[local]
+Arguments builtin_function_symbol (Signature) : clear implicits.
+#[local]
+Arguments builtin_predicate_symbol (Signature) : clear implicits.
+#[local]
+Arguments builtin_function_interp {symbol} {symbols signature}
+  {NondetValue Carrier} (ModelOver) _ _ _
+.
+#[local]
+Arguments builtin_predicate_interp {symbol} {symbols signature}
+  {NondetValue Carrier} (ModelOver) _ _ _
+.
+
+Record SignatureMorphism (s1 s2 : Signature) := {
+    function_symbol_morphism : (builtin_function_symbol s1) -> (builtin_function_symbol s2) ;
+    predicate_symbol_morphism : (builtin_predicate_symbol s1) -> (builtin_predicate_symbol s2) ;
+}.
+
+Arguments function_symbol_morphism {s1 s2} s _.
+Arguments predicate_symbol_morphism {s1 s2} s _.
+
+Class SMInj {s1 s2 : Signature} (μ : SignatureMorphism s1 s2) := {
+    smif :: Inj (=) (=) (function_symbol_morphism μ) ;
+    smip :: Inj (=) (=) (predicate_symbol_morphism μ) ;
+}.
